WIP

Validator/StateSetFormalism/Mods.lean
@@ -1,15 +1,56 @@
 module
 
 public import Validator.StateSetFormalism.Formula
+import Std.Data.HashSet.Lemmas
+
+-- TODO : make more efficient and move to Basic.lean
+
+def Std.HashSet.filterMap {α} [BEq α] [Hashable α] {β} [BEq β] [Hashable β]
+    (f : α → Option β) (m : Std.HashSet α) : Std.HashSet β :=
+  Std.HashSet.ofList (m.toList.filterMap f)
+
+@[simp]
+lemma Std.HashSet.mem_filterMap {α} [BEq α] [Hashable α] [LawfulBEq α] [LawfulHashable α]
+    {β} [BEq β] [Hashable β] [LawfulBEq β] [LawfulHashable β]
+    {f : α → Option β} {m : Std.HashSet α} {b : β} :
+    b ∈ m.filterMap f ↔ ∃ a ∈ m, f a = some b := by
+  simp only [filterMap, mem_ofList, List.contains_eq_mem, List.mem_filterMap, mem_toList,
+    decide_eq_true_eq]
+
+def Std.HashSet.biUnion {α} [BEq α] [Hashable α] {β} [BEq β] [Hashable β]
+    (f : α → Std.HashSet β) (m : Std.HashSet α) : Std.HashSet β :=
+  Std.HashSet.ofList (m.toList.flatMap fun m ↦ (f m).toList)
+
+@[simp]
+lemma Std.HashSet.mem_flatMap {α} [BEq α] [Hashable α] [LawfulBEq α] [LawfulHashable α]
+    {β} [BEq β] [Hashable β] [LawfulBEq β] [LawfulHashable β]
+    {f : α → Std.HashSet β} {m : Std.HashSet α} {b : β} :
+    b ∈ m.biUnion f ↔ ∃ a ∈ m, b ∈ f a := by
+  simp only [biUnion, mem_ofList, List.contains_eq_mem, List.mem_flatMap, mem_toList,
+    decide_eq_true_eq]
+
+def Std.HashSet.attachMap {α} [BEq α] [LawfulBEq α] [Hashable α] {β} [BEq β] [Hashable β]
+     (m : Std.HashSet α) (f : (a : α) → a ∈ m → β): Std.HashSet β :=
+  Std.HashSet.ofList (m.toList.attach.map fun ⟨a, ha⟩ ↦ f a (Std.HashSet.mem_toList.1 ha))
+
+@[simp]
+lemma Std.HashSet.mem_attachMap {α} [BEq α] [Hashable α] [LawfulBEq α] [LawfulHashable α]
+    {β} [BEq β] [Hashable β] [LawfulBEq β] [LawfulHashable β]
+    {m : Std.HashSet α} {f : (a : α) → a ∈ m → β} {b : β} :
+    b ∈ m.attachMap f ↔ ∃ a ha, f a ha = b := by
+  simp only [attachMap, mem_ofList, List.contains_eq_mem, List.mem_map, List.mem_attach, true_and,
+    Subtype.exists, mem_toList, decide_eq_true_eq]
 
 namespace Validator
 open Formula STRIPS
 
+public instance {n} : Hashable (PartialModel n) where
+  hash M := mixHash (hash M.pos.toBitVec) (hash M.neg.toBitVec)
+
 public structure MODS n where
   private vars : VarSet n
-  private mods : List (PartialModel n)
-  private prop : ∀ M ∈ mods, M.vars = vars
-  deriving DecidableEq
+  private mods : Std.HashSet (PartialModel n)
+  private vars_eq : ∀ M ∈ mods, M.vars = vars
 
 namespace PartialModel
 
@@ -51,6 +92,263 @@ lemma isSome_and_iff {n} {M1 M2 : PartialModel n} :
     use fun i ↦ i ∈ M1.pos ∨ i ∈ M2.pos
     grind only
   · grind only
+
+def restrict {n} (M : PartialModel n) (vars : VarSet n) : PartialModel n where
+  pos := M.pos ∩ vars
+  neg := M.neg ∩ vars
+  disjoint := by grind only [VarSet.inter_eq_empty_iff, VarSet.mem_inter, M.disjoint]
+
+@[simp]
+lemma pos_restrict {n} {M : PartialModel n} {vars} : (M.restrict vars).pos = M.pos ∩ vars := rfl
+
+@[simp]
+lemma neg_restrict {n} {M : PartialModel n} {vars} : (M.restrict vars).neg = M.neg ∩ vars := rfl
+
+@[simp]
+lemma vars_restrict {n} {M : PartialModel n} {vars} : (M.restrict vars).vars = M.vars ∩ vars := by
+  ext i
+  grind only [vars_eq, !pos_restrict, !neg_restrict, VarSet.mem_inter, VarSet.mem_union]
+
+@[simp]
+lemma mem_restrict {n} {M : PartialModel n} {vars l} :
+    l ∈ M.restrict vars ↔ l ∈ M ∧ l.var ∈ vars := by
+  grind only [restrict, mem_iff, VarSet.mem_inter]
+
+lemma models_subset_models_restrict {n} {M : PartialModel n} {vars} :
+    M.models ⊆ (M.restrict vars).models := by
+  simp only [Set.subset_def, mem_models', pos_restrict, VarSet.mem_inter, and_imp, neg_restrict]
+  grind only
+
+@[simp]
+lemma restrict_inter {n} {M : PartialModel n} {V1 V2} :
+    M.restrict (V1 ∩ V2) = (M.restrict V1).restrict V2 := by
+  rw [PartialModel.ext'_iff]
+  grind only [mem_restrict, VarSet.mem_inter]
+
+@[simp]
+lemma restrict_vars_eq_self_iff {n} {M : PartialModel n} {vars} :
+    M.restrict vars = M ↔ M.vars ⊆ vars := by
+  simp only [PartialModel.ext_iff, pos_restrict, VarSet.ext_iff, VarSet.mem_inter,
+    neg_restrict, vars_eq, VarSet.subset_iff, VarSet.mem_union]
+  grind only
+
+@[simp]
+lemma restrict_vars_self {n} {M : PartialModel n} : M.restrict M.vars = M := by
+  simp only [restrict_vars_eq_self_iff, VarSet.subset_iff, imp_self, implies_true]
+
+/--
+If two partial models `M1` and `M2` agree on their common variables,
+then their conjunction is well-defined.
+-/
+lemma exists_of_restrict_eq {n} {M1 M2 : PartialModel n} :
+    M1.restrict M2.vars = M2.restrict M1.vars → ∃ M3 : PartialModel n, M1.and M2 = some M3 := by
+  intro h1
+  rw [← Option.isSome_iff_exists ,isSome_and_iff]
+  simp only [ne_eq, ← Set.nonempty_iff_ne_empty]
+  use fun i ↦ i ∈ M1.pos ∨ i ∈ M2.pos
+  simp only [Set.mem_inter_iff, mem_models', not_or]
+  simp only [PartialModel.ext_iff, pos_restrict, neg_restrict, PartialModel.vars_eq] at h1
+  simp only [VarSet.ext_iff, VarSet.mem_inter, VarSet.mem_union] at h1
+  grind only [VarSet.inter_eq_empty_iff, M1.disjoint, M2.disjoint]
+
+/--
+If two partial models `M1` and `M2` agree on their common variables,
+then their conjunction is well-defined.
+-/
+lemma exists_iff_restrict_eq {n} {M1 M2 : PartialModel n} :
+    M1.restrict M2.vars = M2.restrict M1.vars ↔ ∃ M3 : PartialModel n, M1.and M2 = some M3 := by
+  rw [← Option.isSome_iff_exists ,isSome_and_iff]
+  simp only [ne_eq, ← Set.nonempty_iff_ne_empty]
+  simp only [PartialModel.ext_iff, pos_restrict, neg_restrict, PartialModel.vars_eq]
+  simp only [VarSet.ext_iff, VarSet.mem_inter, VarSet.mem_union]
+  constructor
+  · intro h1
+    use fun i ↦ i ∈ M1.pos ∨ i ∈ M2.pos
+    simp only [Set.mem_inter_iff, mem_models', not_or]
+    grind only [VarSet.inter_eq_empty_iff, M1.disjoint, M2.disjoint]
+  · rintro ⟨M, hM⟩
+    simp only [Set.mem_inter_iff, mem_models'] at hM
+    grind only [VarSet.inter_eq_empty_iff, M1.disjoint, M2.disjoint]
+
+/--
+If two partial models `M1` and `M2` agree on their common variables,
+then their conjunction is well-defined.
+-/
+lemma restrict_eq_iff {n} {M1 M2 : PartialModel n} :
+    M1.restrict M2.vars = M2.restrict M1.vars ↔ M1.models ∩ M2.models ≠ ∅ := by
+  simp only [ne_eq, ← Set.nonempty_iff_ne_empty]
+  simp only [PartialModel.ext_iff, pos_restrict, neg_restrict, PartialModel.vars_eq]
+  simp only [VarSet.ext_iff, VarSet.mem_inter, VarSet.mem_union]
+  constructor
+  · intro h1
+    use fun i ↦ i ∈ M1.pos ∨ i ∈ M2.pos
+    simp only [Set.mem_inter_iff, mem_models', not_or]
+    grind only [VarSet.inter_eq_empty_iff, M1.disjoint, M2.disjoint]
+  · rintro ⟨M, hM⟩
+    simp only [Set.mem_inter_iff, mem_models'] at hM
+    grind only [VarSet.inter_eq_empty_iff, M1.disjoint, M2.disjoint]
+
+/--
+Expand the given partial model `M` to `2 ^ |Varset.ofList xs|` partial models over
+`M.vars ∪ Varset.ofList xs`.
+-/
+-- TODO : implement iterator for `VarSet` and use it here instead of `List`
+def expand' {n} (M : PartialModel n) (xs : List (Fin n))
+    (h1 : xs.Nodup) (h2 : ∀ x ∈ xs, x ∉ M.vars) : List (PartialModel n) :=
+  match xs with
+  | [] => [M]
+  | x :: xs' =>
+    let M1 := M.insert ⟨x, false⟩ (by grind only [= List.mem_cons])
+    let M2 := M.insert ⟨x, true⟩ (by grind only [= List.mem_cons])
+    have hM1 : ∀ x ∈ xs', x ∉ M1.vars := by
+      simp only [vars_insert, VarSet.mem_insert, not_or, M1]
+      grind only [= List.nodup_cons, = List.mem_cons]
+    have hM2 : ∀ x ∈ xs', x ∉ M2.vars := by
+      simp only [vars_insert, VarSet.mem_insert, not_or, M2]
+      grind only [= List.nodup_cons, = List.mem_cons]
+    M1.expand' xs' (by grind) hM1 ++ M2.expand' xs' (by grind) hM2
+
+lemma vars_of_mem_expand' {n} {M : PartialModel n} {xs h1 h2} {M' : PartialModel n} :
+    M' ∈ M.expand' xs h1 h2 → M'.vars = M.vars ∪ VarSet.ofList xs := by
+  fun_induction expand' with
+  | case1 M =>
+    grind only [List.mem_cons, !VarSet.ofList_nil, List.not_mem_nil, VarSet.union_empty]
+  | case2 M x xs h1 h2 M1 M2 hM1 hM2 ih1 ih2 =>
+    simp only [List.mem_append, VarSet.ofList_cons]
+    simp [VarSet.ext_iff] at ⊢ ih1 ih2
+    rintro (h3 | h3)
+    · grind only [ih1 h3, vars_insert, VarSet.mem_insert]
+    · grind only [ih2 h3, vars_insert, VarSet.mem_insert]
+
+lemma mem_expand'_aux1 {n} {M M' : PartialModel n} {l hl} :
+    M'.restrict (M.insert l hl).vars = M.insert l hl → M'.restrict M.vars = M := by
+  rintro h1
+  refine ext' (fun l' ↦ ?_)
+  simp only [mem_restrict]
+  if heq : l' = l then
+    grind only [mem_vars]
+  else
+    simp only [PartialModel.ext'_iff, mem_restrict] at h1
+    simp only [vars_insert, VarSet.mem_insert, mem_insert_iff] at h1
+    have h2 := h1 l'.negate
+    specialize h1 l'
+    simp only [Literal.ext_iff, Literal.var_negate, Literal.isPos_negate] at *
+    grind only [not_mem_or_negate_not_mem]
+
+lemma mem_expand'_aux2 {n} {M M' : PartialModel n} {l hl} :
+    M'.restrict M.vars = M → l ∈ M' → M'.restrict (M.insert l hl).vars = M.insert l hl := by
+  rintro h1 h2
+  refine ext' (fun l' ↦ ?_)
+  simp only [vars_insert, mem_restrict, VarSet.mem_insert, mem_insert_iff]
+  if heq : l' = l then
+    grind only
+  else
+    simp only [PartialModel.ext'_iff, mem_restrict] at h1
+    simp only [← h1 l', heq, or_false, and_congr_right_iff, or_iff_left_iff_imp]
+    grind only [not_mem_or_negate_not_mem, Literal.eq_or_eq_negate_iff_var_eq]
+
+lemma mem_expand' {n} {M : PartialModel n} {xs h1 h2} {M' : PartialModel n} :
+    M' ∈ M.expand' xs h1 h2 ↔ M'.vars = M.vars ∪ VarSet.ofList xs ∧ M'.restrict M.vars = M := by
+  constructor
+  · intro h3
+    simp only [vars_of_mem_expand' h3, true_and]
+    fun_induction expand' with
+    | case1 M =>
+      simp only [List.mem_cons, List.not_mem_nil, or_false] at h3
+      simp only [← h3, restrict_vars_eq_self_iff]
+      grind only
+    | case2 M x xs h1 h2 M1 M2 hM1 hM2 ih1 ih2 =>
+      simp only [List.mem_append] at h3
+      rcases h3 with (h3 | h3)
+      · exact mem_expand'_aux1 (ih1 h3)
+      · exact mem_expand'_aux1 (ih2 h3)
+  · rintro ⟨h3, h4⟩
+    fun_induction expand' with
+    | case1 M =>
+      simp only [List.mem_cons, List.not_mem_nil, or_false]
+      simp only [VarSet.ofList_nil, VarSet.union_empty] at h3
+      symm
+      rw [← h4, restrict_vars_eq_self_iff, h3]
+      grind only
+    | case2 M x xs h1 h2 M1 M2 hM1 hM2 ih1 ih2 =>
+      simp only [List.mem_append]
+      simp only [VarSet.ofList_cons, VarSet.ext_iff, VarSet.mem_union, VarSet.mem_insert,
+        VarSet.mem_ofList] at h3
+      have h5 : M'.vars = VarSet.insert x M.vars ∪ VarSet.ofList xs := by
+        simp only [VarSet.ext_iff, VarSet.mem_union, VarSet.mem_insert, VarSet.mem_ofList]
+        grind only
+      specialize ih1 (by simp only [h5, vars_insert, M1])
+      specialize ih2 (by simp only [h5, vars_insert, M2])
+      specialize h3 x
+      simp only [or_true, iff_true, PartialModel.mem_vars] at h3
+      rcases h3 with ⟨l, hl, rfl⟩
+      cases h6 : l.isPos with
+      | false => exact .inl <| ih1 <| mem_expand'_aux2 h4 (by simp only [← h6, hl])
+      | true => exact .inr <| ih2 <| mem_expand'_aux2 h4 (by simp only [← h6, hl])
+
+/-- Expand the given partial model `M` to `2 ^ |V \ M.vars|` partial models over `M.vars ∪ V`. -/
+-- TODO : implement this as an iterator, as `Implicant` only needs to check a linear amount of
+-- partial models, avoiding the exponential complexity
+def expand {n} (M : PartialModel n) (V : VarSet n) : List (PartialModel n) :=
+  M.expand' (V \ M.vars).toList VarSet.toList_nodup (by simp)
+
+lemma vars_of_mem_expand {n} {M : PartialModel n} {V} {M' : PartialModel n} :
+    M' ∈ M.expand V → M'.vars = M.vars ∪ V := by
+  intro h
+  have := vars_of_mem_expand' h
+  simp_all only [VarSet.ofList_toList, VarSet.ext_iff, VarSet.mem_union, VarSet.mem_diff]
+  grind only
+
+lemma mem_expand {n} {M : PartialModel n} {V} {M' : PartialModel n} :
+    M' ∈ M.expand V ↔ M'.vars = M.vars ∪ V ∧ M'.restrict M.vars = M := by
+  simp only [expand, mem_expand', VarSet.ofList_toList, VarSet.ext_iff, VarSet.mem_union,
+    VarSet.mem_diff, and_congr_left_iff]
+  grind only
+
+lemma expand_restrict {n} {M : PartialModel n} {V} {M'} :
+    M' ∈ (M.restrict V).expand V ↔ ∃ M'' ∈ M.expand V, M''.restrict V = M' := by
+  simp only [mem_expand, vars_restrict]
+  constructor
+  · intro ⟨h1, h2⟩
+    obtain ⟨rfl⟩ : M'.vars = V := by
+      simp_all only [VarSet.ext_iff, VarSet.mem_union, VarSet.mem_inter]
+      tauto
+    rw [VarSet.inter_comm, restrict_inter, restrict_vars_self, exists_iff_restrict_eq] at h2
+    rcases h2 with ⟨M'', h2⟩
+    use M''
+    rw [vars_and h2, VarSet.union_comm]
+
+    sorry
+  · rintro ⟨M'', ⟨h1, h2⟩, rfl⟩
+    have h : V ∩ (M.vars ∩ V) = M.vars ∩ V := by
+      simp [VarSet.ext_iff, VarSet.mem_inter]
+    rw [← restrict_inter, h, restrict_inter, h2]
+    simp only [vars_restrict, h1, VarSet.ext_iff, VarSet.mem_inter, VarSet.mem_union, and_true]
+    grind only
+
+
+lemma subset_models_of_expand {n} {M : PartialModel n} {V} :
+    ∀ M' ∈ M.expand V, M'.models ⊆ M.models := by
+  simp only [mem_expand]
+  intro M' ⟨h1, h2⟩ M'' h3
+  simp only [mem_models'] at ⊢ h3
+  simp only [PartialModel.ext_iff, pos_restrict, VarSet.ext_iff, VarSet.mem_inter,
+    neg_restrict] at h2
+  grind only
+
+lemma models_expand {n} (M : PartialModel n) V :
+    M.models = ⋃ M' ∈ M.expand V, M'.models := by
+  ext M1
+  simp only [Set.mem_iUnion, mem_expand, exists_prop]
+  constructor
+  · intro hM1
+    use M
+    sorry
+  · rintro ⟨M', ⟨h1, h2⟩, h3⟩
+    simp only [mem_models'] at ⊢ h3
+    simp only [PartialModel.ext_iff, pos_restrict, VarSet.ext_iff, VarSet.mem_inter,
+      neg_restrict] at h2
+    grind only
 
 /-
 lemma disjoint {n} {V : VarSet n} {M1 M2 : PartialModel V} {M} :
@@ -94,9 +392,9 @@ lemma isTrivial_iff' {n} {γ : Clause n} : isTrivial γ ↔ ∃ l ∈ γ, l.nega
   simp only [isTrivial, Vector.mem_iff_getElem', Fin.getElem_fin, getElem_isTrivial_aux,
     Vector.getElem_replicate, Bool.true_eq_false, decide_false, Bool.false_or, decide_eq_true_eq]
   constructor
-  · grind [Literal.negate]
+  · grind only [Literal.negate_eq]
   · rintro ⟨⟨v, (true | false)⟩, h⟩
-    all_goals grind [Literal.negate]
+    all_goals grind only [Literal.negate_eq]
 
 lemma isTrivial_iff {n} {γ : Clause n} : isTrivial γ ↔ γ.models = Set.univ := by
   sorry
@@ -115,6 +413,52 @@ def models {n} (φ : MODS n) : Models n :=
 lemma mem_models {n} {φ : MODS n} {M} : M ∈ φ.models ↔ ∃ M' ∈ φ.mods, M ∈ M'.models := by
   simp [models]
 
+lemma restrict_mem_mods {n} {φ : MODS n} {M : PartialModel n} (h : φ.vars ⊆ M.vars) :
+    M.restrict φ.vars ∈ φ.mods ↔ M.models ⊆ φ.models := by
+  simp only [Set.subset_def, mem_models]
+  constructor
+  · grind only [PartialModel.mem_models', !PartialModel.pos_restrict, !PartialModel.neg_restrict,
+      VarSet.mem_inter]
+  · intro h'
+    have h1 : ∀ i ∈ M.neg, i ∉ M.pos := by
+      grind only [VarSet.inter_eq_empty_iff, M.disjoint]
+    specialize h' (fun i ↦ i ∈ M.pos) (by grind only [PartialModel.mem_models'])
+    rcases h' with ⟨M', h2, h3⟩
+    have h4 : M.restrict φ.vars = M' := by
+      simp [PartialModel.mem_models'] at h3
+      rw [← φ.vars_eq M' h2] at ⊢ h
+      ext i
+      · grind only [PartialModel.vars_eq, !PartialModel.pos_restrict, VarSet.mem_inter,
+          VarSet.mem_union]
+      · have : ∀ i ∈ M'.neg, i ∈ M.neg := by
+          simp only [PartialModel.vars_eq, VarSet.subset_iff, VarSet.mem_union] at h
+          grind only
+        grind only [PartialModel.vars_eq, !PartialModel.neg_restrict, VarSet.mem_inter,
+          VarSet.mem_union]
+    simp only [h4, h2]
+
+lemma models_subset_models_iff {n} {φ : MODS n} {M : PartialModel n} :
+    M.models ⊆ φ.models ↔ ∀ M' ∈ (M.restrict φ.vars).expand φ.vars, M' ∈ φ.mods := by
+  simp only [PartialModel.expand_restrict, forall_exists_index, and_imp, forall_apply_eq_imp_iff₂]
+  constructor
+  · intro h1 M' hM'
+    have h2 := PartialModel.subset_models_of_expand M' hM'
+    have h3 := Set.Subset.trans h2 h1
+    have h4 : φ.vars ⊆ M'.vars := by
+      rw [PartialModel.vars_of_mem_expand hM']
+      simp only [VarSet.subset_iff, VarSet.mem_union]
+      tauto
+    rwa [← restrict_mem_mods h4] at h3
+  · rw [M.models_expand φ.vars]
+    intro h1 M' hM'
+    simp only [Set.mem_iUnion, exists_prop] at hM'
+    rcases hM' with ⟨M'', h2, hM'⟩
+    specialize h1 M'' h2
+    rw [PartialModel.mem_expand] at h2
+    simp only [mem_models]
+    grind only [PartialModel.mem_models', !PartialModel.pos_restrict, !PartialModel.neg_restrict,
+      VarSet.mem_inter]
+
 @[no_expose]
 public instance {n} : Formula n (MODS n) where
 
@@ -126,29 +470,30 @@ public instance {n} : Formula n (MODS n) where
     simp only [mem_models, PartialModel.mem_models, Literal.mem_models]
     rintro h1 ⟨M'', h2, h3⟩
     use M'', h2
-    have h4 := φ.prop M'' h2
+    have h4 := φ.vars_eq M'' h2
     simp only [← h4, PartialModel.mem_vars] at h1
     grind only
 
 @[no_expose]
 public instance {n} : Top n (MODS n) where
 
-  top := ⟨∅, [PartialModel.empty], by simp⟩
+  top := ⟨∅, {PartialModel.empty}, by simp⟩
 
   models_top := by
-    simp only [Formula.models, Set.eq_univ_iff_forall, mem_models, List.mem_cons, List.not_mem_nil,
-      or_false, exists_eq_left, PartialModel.models_empty, Set.mem_univ, implies_true]
+    simp only [Formula.models, Std.HashSet.singleton_eq_insert, Set.eq_univ_iff_forall, mem_models,
+      Std.HashSet.mem_insert, beq_iff_eq, Std.HashSet.not_mem_empty, or_false, exists_eq_left',
+      PartialModel.models_empty, Set.mem_univ, implies_true]
 
 @[no_expose]
 public instance {n} : Bot n (MODS n) where
 
-  bot := ⟨∅, [], by simp⟩
+  bot := ⟨∅, ∅, by simp⟩
 
   vars_bot := by simp only [Formula.vars]
 
   models_bot := by
-    simp only [Formula.models, Set.eq_empty_iff_forall_notMem, mem_models, List.not_mem_nil,
-      false_and, exists_false, not_false_eq_true, implies_true]
+    simp only [Formula.models, Set.eq_empty_iff_forall_notMem, mem_models,
+      Std.HashSet.not_mem_empty, false_and, exists_false, not_false_eq_true, implies_true]
 
 @[no_expose]
 public instance {n} : ClausalEntailment n (MODS n) where
@@ -157,17 +502,16 @@ public instance {n} : ClausalEntailment n (MODS n) where
 
   entails_iff := by
     intro φ γ
-    simp only [Bool.or_eq_true, List.all_eq_true, List.any_eq_true, decide_eq_true_eq,
-      Formula.models, Set.subset_def, mem_models, forall_exists_index, and_imp]
+    simp only [Bool.or_eq_true, Std.HashSet.all_eq_true_iff_forall_mem, List.any_eq_true,
+      decide_eq_true_eq, Formula.models, Set.subset_def, mem_models, forall_exists_index, and_imp]
     constructor
     · intro h M M' hM' hM
       rcases h with h | h
-      · obtain ⟨i, hi, rfl⟩ := List.getElem_of_mem hM'
-        specialize h φ.mods[i] hM'
+      · specialize h M' hM'
         rcases h with ⟨l, h1, h2⟩
         rw [Clause.mem_models]
         use l, h1
-        simp_all only [List.getElem_mem, PartialModel.mem_models]
+        simp_all only [PartialModel.mem_models]
       · rw [Clause.isTrivial_iff, Set.eq_univ_iff_forall] at h
         exact h M
     · simp only [Clause.mem_models', or_iff_not_imp_right]
@@ -199,33 +543,50 @@ public instance {n} : ClausalEntailment n (MODS n) where
         · simp_all
           specialize h3 _ h1
           specialize h2 _ h1
-          grind only [Literal.negate, PartialModel.mem_iff]
+          grind only [Literal.negate_eq, PartialModel.mem_iff]
       specialize h1 M' M hM h4 h2
       grind only [Clause.mem_models]
 
 @[no_expose]
 public instance {n} : Implicant n (MODS n) where
 
-  entails δ φ := sorry
+  entails δ φ := match δ.toPartialModel with
+    | some M =>
+      if φ.vars ⊆ M.vars then
+        M.restrict φ.vars ∈ φ.mods
+      else
+        M.restrict φ.vars |>.expand φ.vars |>.all (· ∈ φ.mods)
+    | none => true
 
-  entails_iff := sorry
+  entails_iff δ φ := by
+    simp only [Formula.models]
+    split
+    next M h1 =>
+      rw [← Cube.models_toPartialModel h1]
+      split
+      next h2 => simp only [restrict_mem_mods h2, decide_eq_true_eq]
+      next h2 => simp only [List.all_eq_true, decide_eq_true_eq, models_subset_models_iff]
+    next h =>
+      rw [Cube.toPartialModel_eq_none_iff] at h
+      simp only [h, Set.empty_subset]
 
 @[no_expose]
 public instance {n} : BoundedConjuction n (MODS n) where
 
   and φ ψ := {
     vars := φ.vars ∪ ψ.vars
-    mods := φ.mods.flatMap fun δ ↦ ψ.mods.filterMap fun δ' ↦ δ.and δ'
-    prop := by
-      simp only [List.mem_flatMap, List.mem_filterMap, forall_exists_index, and_imp]
+    mods :=
+      φ.mods.biUnion fun δ ↦ ψ.mods.filterMap fun δ' ↦ δ.and δ'
+    vars_eq := by
+      simp only [Std.HashSet.mem_flatMap, Std.HashSet.mem_filterMap, forall_exists_index, and_imp]
       intro M M1 h1 M2 h2
-      rw [← φ.prop M1 h1, ← ψ.prop M2 h2]
+      rw [← φ.vars_eq M1 h1, ← ψ.vars_eq M2 h2]
       exact PartialModel.vars_and
     }
 
   models_and φ ψ := by
-    simp only [Formula.models, Set.ext_iff, mem_models, List.mem_flatMap, List.mem_filterMap,
-      Set.mem_inter_iff]
+    simp only [Formula.models, Set.ext_iff, mem_models, Std.HashSet.mem_flatMap,
+      Std.HashSet.mem_filterMap, Set.mem_inter_iff]
     intro M
     constructor
     · grind only [→ PartialModel.models_and, = Set.mem_inter_iff]
@@ -238,20 +599,14 @@ public instance {n} : BoundedConjuction n (MODS n) where
       grind only [= Set.mem_inter_iff, PartialModel.models_and hM']
 
 @[no_expose]
-public instance {n} : SententialEntailment n (MODS n) where
-
-  entails φ ψ := sorry
-
-  entails_iff := sorry
-
-@[no_expose]
 public instance {n} : OfPartialModel n (MODS n) where
 
-  ofPartialModel M := ⟨M.vars, [M], by simp⟩
+  ofPartialModel M := ⟨M.vars, {M}, by simp⟩
 
   vars_ofPartialModel := by simp only [Formula.vars, implies_true]
 
-  models_ofPartialModel := by simp only [Formula.models, models, List.mem_singleton, exists_eq_left,
+  models_ofPartialModel := by simp only [Formula.models, models, Std.HashSet.singleton_eq_insert,
+    Std.HashSet.mem_insert, beq_iff_eq, Std.HashSet.not_mem_empty, or_false, exists_eq_left',
     Set.ofPred_mem_eq, implies_true]
 
 @[no_expose]
@@ -259,11 +614,12 @@ public instance {n} : Rename n (MODS n) where
 
   rename φ V r h1 := {
     vars :=  φ.vars.map r.rename
-    mods := φ.mods.attach.map fun ⟨M, hM⟩ ↦ PartialModel.rename r M (φ.prop M hM ▸ h1)
-    prop := by
-      simp only [List.mem_map, List.mem_attach, true_and, Subtype.exists, forall_exists_index]
+    mods :=
+      φ.mods.attachMap fun M hM ↦ PartialModel.rename r M (φ.vars_eq M hM ▸ h1)
+    vars_eq := by
+      simp only [Std.HashSet.mem_attachMap, forall_exists_index]
       intro M' M hM rfl
-      simp only [← φ.prop M hM, SetLike.ext_iff, PartialModel.mem_vars_rename, VarSet.mem_map]
+      simp only [← φ.vars_eq M hM, SetLike.ext_iff, PartialModel.mem_vars_rename, VarSet.mem_map]
       grind only [PartialModel.mem_vars]
     }
 
@@ -284,10 +640,10 @@ public instance {n} : ToCNF n (MODS n) where
 @[no_expose]
 public instance {n} : ToDNF n (MODS n) where
 
-  toDNF φ := φ.mods.map PartialModel.toCube
+  toDNF φ := φ.mods.toList.map PartialModel.toCube
 
   models_toDNF := by
-    simp only [Formula.models, Set.ext_iff, DNF.mem_models, List.mem_map, exists_exists_and_eq_and,
-      PartialModel.models_toCube, mem_models, implies_true]
+    simp only [Formula.models, Set.ext_iff, DNF.mem_models, List.mem_map, Std.HashSet.mem_toList,
+      exists_exists_and_eq_and, PartialModel.models_toCube, mem_models, implies_true]
 
 end Validator.MODS
